Regex/Compiler/Basic.lean
@@ -1,0 +1,37 @@
+import Regex.Syntax.Hir
+import Regex.Nfa
+
+namespace Compiler
+
+open Syntax
+open NFA
+
+/-!
+## Compiler
+
+Compile from a regex's high-level intermediate representation (`Syntax.Hir`)
+into an NFA state graph (`NFA`).
+-/
+
+/-- The configuration used for a Thompson NFA compiler. -/
+structure Config where
+  /-- Whether to compile an unanchored prefix into this NFA. -/
+  unanchored_prefix: Bool
+  /-- Whether to simulate an unanchored prefix with the backtracker. -/
+  unanchored_prefix_simulation : Bool
+
+instance : Inhabited Config := ⟨true, false⟩
+
+/-- A value that represents the result of compiling a sub-expression of a regex's HIR.
+    Specifically, this represents a sub-graph of the NFA that
+    has an initial state at `start` and a final state at `end`.
+-/
+structure ThompsonRef where
+  start: Unchecked.StateID
+  «end»: Unchecked.StateID
+
+instance : ToString ThompsonRef where
+  toString s := s!"{s.start}, {s.end}"
+
+/-- the next `StateID` of all states in array `arr` is less than size of `arr`. -/
+@[simp] def nextOfLt (r : Array Unchecked.State) := ∀ (i : Nat) _, r[i].nextOf < r.size
