Regex/Compiler/Compile.lean
@@ -1,0 +1,596 @@
+import Init.Meta
+import Batteries.Data.Array.Basic
+import Batteries.Lean.Except
+
+import Std.Tactic.Do
+import Std.Tactic.Do.Syntax
+
+import Regex.Syntax.Hir
+import Regex.Nfa
+import Regex.Data.Nat.Basic
+import Regex.Compiler.Basic
+import Regex.Compiler.Patch
+
+namespace Compiler
+
+open Syntax
+open NFA
+
+namespace Code
+
+instance : MonadLiftT (StateT σ Id) (EStateM ε σ) where
+  monadLift := EStateM.modifyGet
+
+instance : MonadLiftT (StateT σ₁ Id) (EStateM ε (σ₁ × σ₂)) where
+  monadLift x := fun s =>
+    let x := (x.run s.1).run
+    EStateM.Result.ok x.1 (x.2, s.2)
+
+instance : MonadLiftT (EStateM ε σ₁) (EStateM ε (σ₁ × σ₂)) where
+  monadLift x := fun s =>
+    match (x.run s.1) with
+    | EStateM.Result.ok x s' => EStateM.Result.ok x (s', s.2)
+    | EStateM.Result.error e s' => EStateM.Result.error e (s', s.2)
+
+/--
+  the state consists of a pair of arrays of capture groups and of Unchecked.State's
+-/
+abbrev CompilerM α := EStateM String (Array Unchecked.State × Array Nat) α
+
+abbrev StackM α := StateT (Array Unchecked.State) Id α
+
+def push (s : Unchecked.State) : StackM Unchecked.StateID := do
+  let states ← get
+  set (states.push s)
+  pure states.size
+
+def push' (s : Unchecked.State) : StackM ThompsonRef := do
+  let states ← get
+  set (states.push s)
+  pure ⟨states.size, states.size⟩
+
+def add_match (pattern_id : PatternID) : StackM Unchecked.StateID :=
+  push (Unchecked.State.Match pattern_id)
+
+def add_union : StackM Unchecked.StateID :=
+  push (Unchecked.State.Union #[])
+
+def add_union_reverse : StackM Unchecked.StateID :=
+  push (Unchecked.State.UnionReverse #[])
+
+def add_backrefence (case_insensitive : Bool) (b : Nat) : StackM Unchecked.StateID :=
+  push (Unchecked.State.BackRef b case_insensitive 0)
+
+def c_range (start «end» : UInt32) : StackM ThompsonRef :=
+  let trans: Unchecked.Transition := ⟨start, «end», 0⟩
+  push' (Unchecked.State.ByteRange trans)
+
+def add_empty : StackM Unchecked.StateID :=
+  push (Unchecked.State.Empty 0)
+
+def add_fail : StackM Unchecked.StateID :=
+  push (Unchecked.State.Fail)
+
+def add_eat (mode : Unchecked.EatMode) : StackM Unchecked.StateID :=
+  push (Unchecked.State.Eat mode 0)
+
+def add_change_state : StackM Unchecked.StateID :=
+  push (Unchecked.State.ChangeFrameStep 0 0)
+
+def add_remove_state : StackM Unchecked.StateID :=
+  push (Unchecked.State.RemoveFrameStep 0)
+
+def add_next_char (offset : Nat) : StackM Unchecked.StateID :=
+  push (Unchecked.State.NextChar offset 0)
+
+def c_empty : StackM  ThompsonRef :=
+  push' (Unchecked.State.Empty 0)
+
+def add_sparse (trans : Array Unchecked.Transition) : StackM Unchecked.StateID :=
+  push (Unchecked.State.SparseTransitions trans)
+
+def c_unicode_class (cls : ClassUnicode) : StackM ThompsonRef := do
+  let «end» ← add_empty
+  let trans := cls.set.intervals.map (fun r => ⟨r.fst.val, r.snd.val, «end»⟩)
+  let start ← add_sparse trans
+  pure (ThompsonRef.mk start «end»)
+
+def c_literal (c : Char) : StackM ThompsonRef :=
+  c_range c.val c.val
+
+def c_look (look : Syntax.Look) : StackM ThompsonRef :=
+  match look with
+  | .Start => push' (Unchecked.State.Look NFA.Look.Start 0)
+  | .End => push' (Unchecked.State.Look NFA.Look.End 0)
+  | .EndWithOptionalLF => push' (Unchecked.State.Look NFA.Look.EndWithOptionalLF 0)
+  | .StartLF => push' (Unchecked.State.Look NFA.Look.StartLF 0)
+  | .EndLF => push' (Unchecked.State.Look NFA.Look.EndLF 0)
+  | .StartCRLF => push' (Unchecked.State.Look NFA.Look.StartCRLF 0)
+  | .EndCRLF => push' (Unchecked.State.Look NFA.Look.EndCRLF 0)
+  | .WordUnicode => push' (Unchecked.State.Look NFA.Look.WordUnicode 0)
+  | .WordUnicodeNegate => push' (Unchecked.State.Look NFA.Look.WordUnicodeNegate 0)
+  | .WordStartUnicode => push' (Unchecked.State.Look NFA.Look.WordStartUnicode 0)
+  | .WordEndUnicode => push' (Unchecked.State.Look NFA.Look.WordEndUnicode 0)
+  | .WordStartHalfUnicode => push' (Unchecked.State.Look NFA.Look.WordStartHalfUnicode 0)
+  | .WordEndHalfUnicode => push' (Unchecked.State.Look NFA.Look.WordEndHalfUnicode 0)
+  | .PreviousMatch => push' (Unchecked.State.Look NFA.Look.PreviousMatch 0)
+  | .ClearMatches => push' (Unchecked.State.Look NFA.Look.ClearMatches 0)
+
+def c_cap' (role : Capture.Role) (pattern_id slot: Nat) : StackM Unchecked.StateID :=
+  push (Unchecked.State.Capture role 0 0 pattern_id slot)
+
+/-- embed `start` to `end` in a possessive union,
+    i.e. remove backtracking frames from stack if `end` state is reached
+-/
+def c_possessive (tref : ThompsonRef) : PatchM ThompsonRef := do
+  let  union ← add_union
+  let  fail ← add_fail
+  let  eat ← add_eat (Unchecked.EatMode.ToLast 0)
+  let  empty ← add_empty
+
+  Code.patch union tref.start
+  Code.patch tref.«end» eat
+  Code.patch union fail
+  Code.patch eat fail
+  Code.patch eat empty
+  pure (ThompsonRef.mk union empty)
+
+def is_possible_empty_repetition (hir : Hir) : Bool :=
+  match hir with
+  | ⟨.Repetition ⟨0, _, _, _, _⟩, _⟩ => true
+  | _ => false
+
+def is_empty_concat (hir : Hir) : Bool :=
+  match hir with
+  | ⟨.Concat #[], _⟩ => true
+  | _ => false
+
+/-- collect group if `hir` is a capture group which may match with a empty string,
+    it is used to build a greedy search in the Pcre flavor -/
+def get_possible_empty_capture_group (hir : Hir) : Option Nat :=
+  let ⟨kind, _⟩ := hir
+  match kind with
+  | .Capture ⟨g, _, ⟨kind, _⟩⟩ =>
+    match kind with
+    | .Repetition ⟨0, _, _, _, _⟩ => some g
+    | .Concat hirs => if hirs.all is_possible_empty_repetition then some g else none
+    | .Alternation hirs => if (hirs.any is_empty_concat) || (hirs.any is_possible_empty_repetition)
+                           then some g else none
+    | _ => none
+  | _ => none
+
+def c_back_ref (case_insensitive : Bool) (n : Nat) : PatchM  ThompsonRef := do
+  let backrefence ← add_backrefence case_insensitive n
+  let empty ← add_empty
+  Code.patch backrefence empty
+  pure (ThompsonRef.mk backrefence empty)
+
+def head (hirs : Array Hir) (h : 0 < hirs.size)
+    : { pair : Hir × Array Hir // pair.1 ∈ hirs ∧ pair.2.size < hirs.size
+                                  ∧ sizeOf pair.2 < sizeOf hirs } :=
+  let l := hirs.toList
+  have : 0 < l.length := by grind
+  match hm : l with | head :: tail => ⟨(head, tail.toArray), by
+    simp
+    have : sizeOf tail < sizeOf l := by simp_all; grind
+    have : sizeOf hirs = 1 + sizeOf hirs.toList := rfl
+    have : head ∈ l := by simp [*]
+    and_intros <;> grind⟩
+
+theorem head_mem_lt {hirs : Array Hir} {h : 0 < hirs.size}
+  (x : { hir // hir ∈ (Code.head hirs h).val.snd })
+    : sizeOf x.val < sizeOf hirs := by
+  have hp := x.property
+  have : sizeOf x.val < sizeOf (head hirs h).val.snd := Array.sizeOf_lt_of_mem hp
+  have : sizeOf (head hirs h).val.snd < sizeOf hirs := by
+    simp [head]
+    split
+    have : sizeOf hirs = 1 + sizeOf hirs.toList := rfl
+    simp +arith [*]
+  grind
+
+theorem head_apply_lt (hirs : Array Hir) (h : 0 < hirs.size)
+    : sizeOf (head hirs h).val.fst < sizeOf hirs := by
+  simp [head]
+  split
+  have : sizeOf hirs = 1 + sizeOf hirs.toList := rfl
+  simp +arith [*]
+
+def cannotMatchEmptyString (hir : Hir) : Bool :=
+  match hir.properties.minimum_len with
+  | some n => n > 0
+  | none => false
+
+def c_lookaround_PositiveLookahead (compiled : ThompsonRef) : PatchM ThompsonRef := do
+  let change_state ← add_change_state
+  let fail ← add_fail
+  let union ← add_union
+  let «end» ← add_empty
+
+  Code.patch compiled.end change_state
+  Code.patch union compiled.start
+  Code.patch change_state fail
+  Code.patch change_state «end»
+  Code.patch union fail
+
+  pure (ThompsonRef.mk union «end»)
+
+def c_lookaround_NegativeLookahead (compiled : ThompsonRef) : PatchM ThompsonRef := do
+  let remove_state ← add_remove_state
+  let empty ← add_empty
+  let union ← add_union
+  let «end» ← add_empty
+
+  Code.patch compiled.end remove_state
+  Code.patch remove_state empty
+  Code.patch union compiled.start
+  Code.patch empty «end»
+  Code.patch union empty
+
+  pure (ThompsonRef.mk union «end»)
+
+def c_lookaround_PositiveLookbehind (next_char : Unchecked.StateID) (compiled : ThompsonRef)
+    : PatchM ThompsonRef := do
+  let «end» ← add_empty
+
+  Code.patch next_char compiled.start
+  Code.patch compiled.end «end»
+
+  pure (ThompsonRef.mk  next_char «end»)
+
+def c_lookaround_NegativeLookbehind (next_char : Unchecked.StateID) (compiled : ThompsonRef)
+    : PatchM ThompsonRef := do
+    let remove_state ← add_remove_state
+    let empty ← add_empty
+    let union ← add_union
+    let «end» ← add_empty
+
+    Code.patch next_char compiled.start
+    Code.patch compiled.end remove_state
+    Code.patch remove_state empty
+    Code.patch union next_char
+    Code.patch empty «end»
+    Code.patch union empty
+
+    pure (ThompsonRef.mk union «end»)
+
+def c_repetition_0_some_1_false (union : Unchecked.StateID) (compiled : ThompsonRef)
+    : PatchM ThompsonRef := do
+  let empty ← add_empty
+  Code.patch union compiled.start
+  Code.patch union empty
+  Code.patch compiled.end empty
+  pure (ThompsonRef.mk union empty)
+
+def c_repetition_0_some_1_true (union : Unchecked.StateID) (compiled : ThompsonRef)
+    : PatchM ThompsonRef := do
+  let eat ← add_eat (Unchecked.EatMode.Until 0)
+  let empty ← add_empty
+  Code.patch union compiled.start
+  Code.patch union empty
+  Code.patch compiled.end eat
+  Code.patch eat empty
+  Code.patch eat empty
+  pure (ThompsonRef.mk union empty)
+
+def c_repetition_0_none (union : Unchecked.StateID) (compiled : ThompsonRef)
+    : PatchM ThompsonRef := do
+  Code.patch union compiled.start
+  Code.patch compiled.end union
+  pure (ThompsonRef.mk union union)
+
+def c_at_least_0_pre (compiled : ThompsonRef) (greedy : Bool) : PatchM Unchecked.StateID := do
+  let plus ← (if greedy then add_union else add_union_reverse)
+  Code.patch compiled.end plus
+  Code.patch plus compiled.start
+  pure plus
+
+def c_at_least_0_post (compiled : ThompsonRef) (plus : Unchecked.StateID) (greedy : Bool)
+  (possessive : Bool) : PatchM ThompsonRef := do
+  let question ← (if greedy then add_union else add_union_reverse)
+  let empty ← add_empty
+  Code.patch question compiled.start
+  Code.patch question empty
+  Code.patch plus empty
+
+  if possessive then c_possessive ⟨question, empty⟩
+  else pure (ThompsonRef.mk question empty)
+
+def c_at_least_set (possible_empty_capture_group : Option Nat) (greedy : Bool) : CompilerM Unit := do
+  let (states, groups) ← get
+  set (states,
+        (match (if greedy then possible_empty_capture_group else none) with
+         | some g => groups.push g
+         | none => groups))
+
+def c_at_least_0 (compiled : ThompsonRef) (possible_empty_capture_group : Option Nat) (greedy : Bool)
+    : CompilerM Unchecked.StateID := do
+  let plus ← c_at_least_0_pre compiled greedy
+  c_at_least_set possible_empty_capture_group greedy
+  pure plus
+
+def c_at_least_1_pre (greedy : Bool) : PatchM Unchecked.StateID := do
+  if greedy then add_union else add_union_reverse
+
+def c_at_least_1_post (compiled : ThompsonRef) (union : Unchecked.StateID)
+  (possessive : Bool) : PatchM ThompsonRef := do
+  Code.patch compiled.end union
+  Code.patch union compiled.start
+
+  if possessive then c_possessive ⟨compiled.start, union⟩
+  else pure (ThompsonRef.mk compiled.start union)
+
+def c_at_least_1 (possible_empty_capture_group : Option Nat) (greedy : Bool)
+    : CompilerM Unchecked.StateID := do
+  let union ← c_at_least_1_pre greedy
+  c_at_least_set possible_empty_capture_group greedy
+  pure union
+
+def c_at_least_2 («prefix» last : ThompsonRef) (greedy : Bool) (possessive : Bool)
+      : PatchM ThompsonRef := do
+  let union ← (if greedy then add_union else add_union_reverse)
+
+  Code.patch «prefix».end last.start
+  Code.patch last.end union
+  Code.patch union last.start
+
+  if possessive then c_possessive  ⟨«prefix».start, union⟩
+  else pure (ThompsonRef.mk «prefix».start union)
+
+def c_bounded.fold.patch.pre (compiled: ThompsonRef) (prev_end : Unchecked.StateID)
+  (greedy : Bool)
+    : PatchM Unchecked.StateID := do
+  let union ← (if greedy then add_union else add_union_reverse)
+  Code.patch prev_end union
+  Code.patch union compiled.start
+  pure union
+
+def c_bounded.fold.patch.possessive (compiled: ThompsonRef) (empty : Unchecked.StateID)
+    : PatchM Unchecked.StateID := do
+  let union ← add_union
+  let fail ← add_fail
+  let eat ← add_eat (Unchecked.EatMode.ToLast 0)
+
+  Code.patch union fail
+  Code.patch eat fail
+  Code.patch eat empty
+
+  pure compiled.end
+
+def c_bounded.fold.patch.post (compiled: ThompsonRef) (union empty : Unchecked.StateID)
+    : PatchM Unchecked.StateID := do
+  Code.patch union empty
+  pure compiled.end
+
+def c_bounded.fold.patch (compiled: ThompsonRef) (prev_end empty : Unchecked.StateID)
+  (greedy : Bool) (possessive : Bool)
+    : PatchM Unchecked.StateID := do
+  let union ← c_bounded.fold.patch.pre compiled prev_end greedy
+  if possessive
+  then c_bounded.fold.patch.possessive compiled empty
+  else c_bounded.fold.patch.post compiled union empty
+
+def c_alt_iter_step (first second : ThompsonRef)
+    : PatchM (Unchecked.StateID × Unchecked.StateID) := do
+  let union ← add_union
+  let «end» ← add_empty
+
+  Code.patch union first.start
+  Code.patch first.end «end»
+  Code.patch union second.start
+  Code.patch second.end «end»
+
+  pure (union, «end»)
+
+def c_rep_pre (greedy : Bool) : PatchM Unchecked.StateID := do
+  if greedy then add_union else add_union_reverse
+
+mutual
+
+def c_concat.fold (hirs : Array Hir) (s : Unchecked.StateID) : CompilerM Unchecked.StateID := do
+  let go (pair : Unchecked.StateID) (hirM : { hir : Hir // hir ∈ hirs }) := do
+    have := Array.sizeOf_lt_of_mem hirM.property
+    let hir ← c hirM.val
+    Code.patch pair hir.start
+    pure hir.end
+  hirs.attach.foldlM go s
+termination_by sizeOf hirs
+
+def c_concat (hirs : Array Hir) : CompilerM ThompsonRef := do
+  match h : hirs.head? with
+  | some (head, tail) =>
+    have : sizeOf head < sizeOf hirs := Array.sizeOf_head?_of_mem h
+    let ⟨start, «end»⟩ ← c head
+    have : sizeOf tail < sizeOf hirs := Array.sizeOf_head?_of_tail h
+    let hir ← c_concat.fold tail «end»
+    pure (ThompsonRef.mk start hir)
+  | none => c_empty
+termination_by sizeOf hirs
+
+def c_alt_iter.fold (hirs : Array Hir) (union «end» : Unchecked.StateID)
+    : CompilerM Unit := do
+  hirs.attach.foldlM (init := ())
+    (fun s ⟨hir, h⟩  => do
+      have : sizeOf hir < sizeOf hirs := Array.sizeOf_lt_of_mem h
+      let compiled ← c hir
+      Code.patch union compiled.start
+      Code.patch compiled.end «end»
+      pure s)
+termination_by sizeOf hirs
+
+def c_alt_iter (hirs : Array Hir) : CompilerM ThompsonRef := do
+  match hHead : hirs.head? with
+  | some (first, tail) =>
+    have : sizeOf tail < sizeOf hirs := Array.sizeOf_head?_of_tail hHead
+    match hTail : tail.head? with
+    | some (second, tail') =>
+      have : sizeOf first < sizeOf hirs := Array.sizeOf_head?_of_mem hHead
+      let first ← c first
+      have : sizeOf second < sizeOf tail := Array.sizeOf_head?_of_mem hTail
+      let second ← c second
+      let (union, «end») ← c_alt_iter_step first second
+      have : sizeOf tail' < sizeOf tail := Array.sizeOf_head?_of_tail hTail
+      c_alt_iter.fold tail' union «end»
+      pure (ThompsonRef.mk union «end»)
+    | none => .error "c_alt_iter, size > 1 expected"
+  | none => .error "c_alt_iter, size > 0 expected"
+termination_by sizeOf hirs
+
+def c_exactly.fold (hir : Hir) (n : Nat) («end» : Unchecked.StateID)
+    : CompilerM Unchecked.StateID := do
+  if 0 < n then
+    (List.replicate n 0).foldlM (init := («end»))
+      (fun s _ => do
+        let ref ← c hir
+        Code.patch s ref.start
+        pure ref.end)
+  else pure («end»)
+termination_by sizeOf hir + sizeOf n
+
+def c_exactly (hir : Hir) (n : Nat) : CompilerM ThompsonRef := do
+  if 0 < n then
+    let ⟨start, «end»⟩ ← c hir
+    let s ← c_exactly.fold hir (n-1) «end»
+    pure (ThompsonRef.mk start s)
+  else c_empty
+termination_by sizeOf hir + sizeOf n
+
+/-- Compile the given expression such that it may be matched `n` or more times -/
+def c_at_least (hir : Hir) (n : Nat) (greedy : Bool) (possessive : Bool)
+    : CompilerM ThompsonRef := do
+  let possible_empty_capture_group := get_possible_empty_capture_group hir
+  if n = 0 then
+    /- compile x* as (x+)?, which preserves the correct preference order if x can match the empty string. -/
+    let compiled ← c hir
+    let plus ← c_at_least_0 compiled possible_empty_capture_group greedy
+    c_at_least_0_post compiled plus greedy possessive
+  else if n = 1 then
+    let compiled ← c hir
+    let union ← c_at_least_1 possible_empty_capture_group greedy
+    c_at_least_1_post compiled union possessive
+  else
+    let «prefix» ← c_exactly hir (n-1)
+    let last ← c hir
+    c_at_least_2 «prefix» last greedy possessive
+termination_by sizeOf hir + sizeOf n + 1
+
+def c_bounded.fold (hir : Hir) (n : Nat) («prefix» : ThompsonRef) (empty : Unchecked.StateID)
+  (greedy : Bool) (possessive : Bool)
+    : CompilerM Unchecked.StateID := do
+  if 0 < n then
+    (List.replicate n 0).foldlM (init := «prefix».end)
+      (fun prev_end _ => do
+        let compiled ← c hir
+        c_bounded.fold.patch compiled prev_end empty greedy possessive)
+  else pure «prefix».end
+termination_by sizeOf hir + sizeOf n
+
+/-- Compile the given expression such that it matches at least `min` times,
+    but no more than `max` times.-/
+def c_bounded (hir : Hir) (min max : Nat) (greedy : Bool) (possessive : Bool)
+    : CompilerM ThompsonRef := do
+  if 0 < max then
+    let «prefix»  ← c_exactly hir min
+    if min = max then
+      if possessive then c_possessive «prefix»
+      else pure (ThompsonRef.mk «prefix».start «prefix».end)
+    else
+      let empty ← add_empty
+      let prev_end ← c_bounded.fold hir (max-min) «prefix» empty greedy possessive
+      Code.patch prev_end empty
+      pure (ThompsonRef.mk «prefix».start empty)
+  else c_empty
+termination_by sizeOf hir + sizeOf min + sizeOf (max - min) + 1
+
+def c_lookaround (look : Lookaround) : CompilerM ThompsonRef := do
+  match look with
+  | .PositiveLookahead h =>
+    let compiled ← c h
+    c_lookaround_PositiveLookahead compiled
+  | .NegativeLookahead h =>
+    let compiled ← c h
+    c_lookaround_NegativeLookahead compiled
+  | .PositiveLookbehind length h =>
+    let next_char ← add_next_char length
+    let compiled ← c h
+    c_lookaround_PositiveLookbehind next_char compiled
+  | .NegativeLookbehind length h =>
+    let next_char ← add_next_char length
+    let compiled ← c h
+    c_lookaround_NegativeLookbehind next_char compiled
+termination_by sizeOf look
+
+def c_repetition (rep : Repetition) : CompilerM ThompsonRef := do
+  match rep with
+  | .mk 0 (some 1) greedy false h => do
+      let union ← c_rep_pre greedy
+      let compiled ← c h
+      c_repetition_0_some_1_false union compiled
+  | .mk 0 (some 1) _ true h => do
+      let union ← add_union
+      let compiled ← c h
+      c_repetition_0_some_1_true union compiled
+  | .mk min none greedy possessive sub => do
+      if min = 0 && cannotMatchEmptyString sub
+      then
+        let union ← c_rep_pre greedy
+        let compiled ← c sub
+        c_repetition_0_none union compiled
+      else c_at_least sub min greedy possessive
+  | .mk min (some max) greedy possessive sub =>
+      if min ≤ max then c_bounded sub min max greedy possessive else c_empty
+termination_by sizeOf rep
+
+def c_cap (hir : Capture) : CompilerM ThompsonRef := do
+  match hir with
+    | .mk pattern_id _ sub =>
+      let start ← c_cap' Capture.Role.Start pattern_id (pattern_id * 2)
+      let «inner» ← c sub
+      let «end» ← c_cap' Capture.Role.End pattern_id (pattern_id * 2 + 1)
+      Code.patch start inner.start
+      Code.patch inner.end «end»
+      pure (ThompsonRef.mk start «end»)
+termination_by sizeOf hir
+
+def c (hir : Hir) : CompilerM ThompsonRef :=
+  have : sizeOf hir.kind < sizeOf hir := Hir.sizeOfKindOfHir hir
+  match h : hir.kind with
+  | .Empty => c_empty
+  | .Literal c => c_literal c
+  | .Class (.Unicode cls) => c_unicode_class cls
+  | .Look look => c_look look
+  | .Lookaround look =>
+    have : sizeOf look < sizeOf hir.kind := by simp [h]
+    c_lookaround look
+  | .BackRef f n => c_back_ref f n
+  | .Repetition rep =>
+    have : sizeOf rep < sizeOf hir.kind := by simp [h]
+    c_repetition rep
+  | .Capture cap =>
+    have : sizeOf cap < sizeOf hir.kind := by simp [h]
+    c_cap cap
+  | .Concat items =>
+    have : sizeOf items < sizeOf hir.kind := by simp [h]
+    c_concat items
+  | .Alternation sub =>
+    have : sizeOf sub < sizeOf hir.kind := by simp [h]
+    c_alt_iter sub
+termination_by sizeOf hir
+
+end
+
+def init (anchored : Bool) : CompilerM ThompsonRef := do
+  let unanchored_prefix ←
+    if anchored then c_empty
+    else c_repetition (Repetition.mk 0 none false false (dot Dot.AnyChar))
+  pure unanchored_prefix
+
+/-- Compile the HIR expression given. -/
+def compile (anchored : Bool) (expr : Hir) : CompilerM Unit := do
+  let unanchored_prefix ← init anchored
+  let one ← c_cap (Capture.mk 0 none expr)
+  let match_state_id ← add_match 0
+  patch one.end match_state_id
+  patch unanchored_prefix.end one.start
+
+end Code
