Regex/Compiler/Patch.lean
@@ -1,0 +1,157 @@
+import Std.Tactic.Do
+import Std.Tactic.Do.Syntax
+
+import Regex.Do.Triple.SpecLemmas
+import Regex.Compiler.Basic
+
+namespace Compiler
+
+open Syntax
+open NFA
+
+namespace Code
+
+abbrev PatchM α := EStateM String (Array Unchecked.State) α
+
+/-- Add a transition from one state to another. -/
+def patch («from» «to» : Unchecked.StateID) : PatchM Unit := do
+  let states ← get
+  if h : «from» < states.size then
+    match hm : states[«from»]'h with
+    | .Empty _ => set (states.set «from» (Unchecked.State.Empty «to») h)
+    | .NextChar offset _ => set (states.set «from» (Unchecked.State.NextChar offset «to») h)
+    | .Fail =>  EStateM.Result.error s!"patch states .Fail unexpected"
+    | .Eat (.Until s) n =>
+        if s = 0
+        then set (states.set «from» (Unchecked.State.Eat (.Until «to») n) h)
+        else if n = 0
+        then set (states.set «from» (Unchecked.State.Eat (.Until s) «to») h)
+        else EStateM.Result.error "patch states, .Eat s and n not null"
+    | .Eat (.ToLast s) n =>
+        if s = 0
+        then set (states.set «from» (Unchecked.State.Eat (.ToLast «to») n) h)
+        else if n = 0 then
+        set (states.set «from» (Unchecked.State.Eat (.ToLast s) «to») h)
+        else EStateM.Result.error "patch states, .Eat s and n not null"
+    | .ChangeFrameStep f t =>
+        if f = 0
+        then set (states.set «from» (Unchecked.State.ChangeFrameStep «to» t) h)
+        else if t = 0
+        then set (states.set «from» (Unchecked.State.ChangeFrameStep f «to»))
+        else EStateM.Result.error "patch states, .ChangeFrameStep from and to not null"
+    | .RemoveFrameStep _ =>
+      set (states.set «from» (Unchecked.State.RemoveFrameStep «to») h)
+    | .Look look _ =>
+      set (states.set «from» (Unchecked.State.Look look «to»))
+    | .BackRef b f _ =>
+      set (states.set «from» (Unchecked.State.BackRef b f «to»))
+    | .ByteRange t =>
+        set (states.set «from» (Unchecked.State.ByteRange {t with «next» := «to»}) h)
+    | .Capture role _ pattern_id group_index slot =>
+        set (states.set «from» (Unchecked.State.Capture role «to» pattern_id group_index slot))
+    | .BinaryUnion alt1 alt2 =>
+        if alt1 = 0
+        then set (states.set «from» (Unchecked.State.BinaryUnion «to» alt2) h)
+        else if alt2 = 0
+        then set (states.set «from» (Unchecked.State.BinaryUnion alt1 «to») h)
+        else EStateM.Result.error "patch states, .BinaryUnion alt1 and alt2 not null"
+    | .SparseTransitions _ => set states
+    | .Union alternates =>
+        set (states.set «from» (Unchecked.State.Union (alternates.push «to»)) h)
+    | .UnionReverse alternates =>
+        set (states.set «from» (Unchecked.State.UnionReverse (alternates.push «to»)) h)
+    | .Match _ => EStateM.Result.error s!"patch states .Match unexpected"
+  else EStateM.Result.error s!"patch index error"
+
+end Code
+
+namespace Lemmas
+
+private theorem all_set_next_of_lt (n : Unchecked.StateID) (s : Unchecked.State)
+  (states : Array Unchecked.State)
+  (h : n < states.size) (hn : Unchecked.State.nextOf s < states.size)
+  (hlt : ∀ (i : Nat) _, states[i].nextOf < states.size)
+    : ∀ (i : Nat) (hi : i < states.size), (((states.set n s h)[i]'(by grind)).nextOf < states.size) := by
+  grind
+
+private theorem eat_lt («from» s : Nat) (n : Unchecked.StateID) (m : Unchecked.EatMode)
+  (states : Array Unchecked.State) (h : «from» < states.size)
+  (hmode : Unchecked.EatMode.nextOf m = s)
+  (hm : states[«from»]'h = Unchecked.State.Eat m n)
+  (hlt : states[«from»].nextOf < states.size)
+    : s < states.size ∧ n < states.size := by
+  rw [hm] at hlt
+  simp [Unchecked.EatMode.nextOf] at hmode
+  unfold Unchecked.State.nextOf at hlt
+  split at hlt <;> try simp_all [Nat.max_lt]
+
+private theorem change_frame_step_lt («from» : Nat) (f t : Unchecked.StateID)
+  (states : Array Unchecked.State) (h : «from» < states.size)
+  (hm : states[«from»]'h = Unchecked.State.ChangeFrameStep f t)
+  (hlt : states[«from»].nextOf < states.size)
+    : f < states.size ∧ t < states.size := by
+  rw [hm] at hlt
+  unfold Unchecked.State.nextOf at hlt
+  grind
+
+private theorem binary_union_lt («from» : Nat) (alt1 alt2 : Unchecked.StateID)
+  (states : Array Unchecked.State) (h : «from» < states.size)
+  (hm : states[«from»]'h = Unchecked.State.BinaryUnion alt1 alt2)
+  (hlt : states[«from»].nextOf < states.size)
+    : alt1 < states.size ∧ alt2 < states.size := by
+  rw [hm] at hlt
+  unfold Unchecked.State.nextOf at hlt
+  grind
+
+private theorem union_lt («from» to : Nat) (alternates : Array Unchecked.StateID)
+  (states : Array Unchecked.State) (h : «from» < states.size)
+  (ht : to < states.size) (hm : states[«from»]'h = Unchecked.State.Union alternates)
+  (hlt : states[«from»].nextOf < states.size)
+    : List.maxD 0 (alternates.toList ++ [to]) < states.size := by
+  rw [hm] at hlt
+  simp +zetaDelta [Unchecked.State.nextOf] at hlt
+  exact List.maxD_of_append_lt hlt ht
+
+private theorem union_reverse_lt («from» to : Nat) (alternates : Array Unchecked.StateID)
+  (states : Array Unchecked.State) (h : «from» < states.size)
+  (ht : to < states.size)
+  (hm : states[«from»]'h = Unchecked.State.UnionReverse alternates)
+  (hlt : states[«from»].nextOf < states.size)
+    : List.maxD 0 (alternates.toList ++ [to]) < states.size := by
+  rw [hm] at hlt
+  simp +zetaDelta [Unchecked.State.nextOf] at hlt
+  exact List.maxD_of_append_lt hlt ht
+
+open Std.Do
+
+set_option mvcgen.warning false
+
+@[spec] theorem patch_spec («from»: Unchecked.StateID) {«to» : Unchecked.StateID}
+  {states : Array Unchecked.State}
+    : ⦃fun s => s = states ∧ nextOfLt states ∧ «from» < states.size ∧ «to» < states.size⦄
+      Code.patch «from» «to»
+      ⦃post⟨fun _ r => states.size = r.size ∧ «to» < r.size ∧ nextOfLt r, fun _ => ⌜True⌝ ⟩⦄ := by
+  mintro _
+  unfold Code.patch
+  mvcgen
+  all_goals simp_all
+  all_goals try intro _ _; expose_names
+  all_goals try (apply all_set_next_of_lt «from» _ states h_1.right.right.left ?_ (h.right.left)); try assumption
+  all_goals try simp_all [Unchecked.State.nextOf, h_1.right.right.right, Nat.max_lt]
+  all_goals try simp [wp]
+  expose_names
+  · simp [eat_lt «from» s_1 n (Unchecked.EatMode.Until s_1)
+      states h_1.right.right.left (by simp_all [Unchecked.EatMode.nextOf]) (by simp_all) (h_1.right.left «from» h_1.right.right.left)]
+  · simp [eat_lt «from» s_1 n (Unchecked.EatMode.Until s_1)
+      states h_1.right.right.left (by simp_all [Unchecked.EatMode.nextOf]) (by simp_all) (h_1.right.left «from» h_1.right.right.left)]
+  · simp [eat_lt «from» s_1 n (Unchecked.EatMode.ToLast 0)
+      states h_1.right.right.left (by simp_all [Unchecked.EatMode.nextOf]) (by simp_all) (h_1.right.left «from» h_1.right.right.left)]
+  · simp [eat_lt «from» s_1 n (Unchecked.EatMode.ToLast s_1)
+      states h_1.right.right.left (by simp_all [Unchecked.EatMode.nextOf]) (by simp_all) (h_1.right.left «from» h_1.right.right.left)]
+  · simp [change_frame_step_lt «from» f t states h_1.right.right.left (by simp_all) (h_1.right.left «from» h_1.right.right.left)]
+  · simp [change_frame_step_lt «from» f t states h_1.right.right.left (by simp_all) (h_1.right.left «from» h_1.right.right.left)]
+  · simp [binary_union_lt «from» alt1 alt2 states h_1.right.right.left (by simp_all) (h_1.right.left «from» h_1.right.right.left)]
+  · simp [binary_union_lt «from» alt1 alt2 states h_1.right.right.left (by simp_all) (h_1.right.left «from» h_1.right.right.left)]
+  · simp [union_lt «from» «to» alternates states (by simp_all) h_1.right.right.right heq (h_1.right.left «from» h_1.right.right.left)]
+  · simp [union_reverse_lt «from» «to» alternates states (by simp_all) h_1.right.right.right heq (h_1.right.left «from» h_1.right.right.left)]
+end Lemmas
