Regex/Do/Triple/SpecLemmas.lean
@@ -1,0 +1,42 @@
+import Std.Tactic.Do
+import Std.Tactic.Do.Syntax
+
+namespace Std.Do
+
+@[spec]
+theorem except_ok_spec {α ε : Type} {x : α} {pre : Prop}
+  {post : α → Prop} {error : ε → Prop}
+  (h : ∀ r, r = x ∧ pre → post r) : ⦃⌜pre⌝⦄ Except.ok x ⦃post⟨fun a => ⌜post a⌝ , fun e => ⌜ error e⌝ ⟩⦄ := by
+  mintro _
+  simp [wp]
+  split
+  · rename_i a heq
+    have : x = a := by simp [Id.run] at heq; assumption
+    simp_all
+  · rename_i heq
+    simp [Id.run] at heq
+
+theorem Except.by_wp {α} {x : α} {prog : Except ε α} (h : prog = Except.ok x)
+  {P : α → Prop} {Q : ε → Prop}
+    : (⊢ₛ wp⟦prog⟧ (fun r => ⌜P r⌝, fun e => ⌜Q e⌝, ())) → P x := by
+    intro hspec
+    simp only [wp, PredTrans.pushExcept_apply, PredTrans.pure_apply] at hspec
+    split at hspec
+    all_goals rename_i heq <;> rw [h, Id.run] at heq <;> simp_all
+
+theorem StateT.by_wp {α σ} {x : α × σ} {s : σ} {prog : StateT σ Id α}
+  (h : StateT.run prog s = x) {P : α → σ → Prop}
+    : (⊢ₛ wp⟦prog⟧ (fun r s => ⌜P r s⌝, ()) s) → P x.1 x.2 := by
+  intro hspec
+  simp only [wp, PredTrans.pure, PredTrans.pushArg_apply, Id.run] at hspec
+  split at hspec
+  simp [StateT.run] at h
+  simp at hspec
+  grind
+
+theorem StateT.Except.by_wp {α σ ε} {x : α × σ} {s : σ} {prog : StateT σ (Except ε) α}
+  (h : prog s = Except.ok x) {P : α → Prop} {Q : ε → Prop}
+    : (⊢ₛ wp⟦prog⟧ (fun r _ => ⌜P r⌝, fun e => ⌜Q e⌝, ()) s) → P x.1 := by
+  intro hspec
+  simp [wp, PredTrans.pure, PredTrans.pushArg_apply, PredTrans.pushExcept, Id.run] at hspec
+  split at hspec <;> simp_all <;> grind
